Updating coq with new take on policies

src/Lazy.v
@@ -2,11 +2,8 @@ Require Import List.
 Import ListNotations.
 Require Import Nat.
 Require Import Bool.
-Require Import Trace.
-Require Import Machine.
-Require Import ObsTrace.
-Require Import TraceProperties.
-Require Import Coroutine.
+
+From StackSafety Require Import Trace Machine ObsTrace TraceProperties Coroutine.
 
 (* A lazy integrity property is one that doesn't care directly about the state
    of the machine, but focuses on whether an adversary can cause changes in the
@@ -17,273 +14,343 @@ Require Import Coroutine.
    The second is slightly stronger, and treats a change to sealed state as a
    secret that should never become observable at all. Its strength avoids certain
    cases where the first property has difficult intuition.
-*)
-Section LAZY_TRACE_PROPS.
-  Variable context : Type.
-  Variable updateC : MachineState -> context -> context.
+ *)
 
-  Definition rollback (m m':MachineState) (K : Component -> Prop) (m'': MachineState) : Prop :=
-    forall k,
-      K k ->
-      m k <> m' k ->
-      m'' k = m k /\
-      (K k \/ m k = m' k) ->
-      m'' k = m' k.
+  Section LAZY_TRACE_PROPS.
 
-  Definition TraceIntegrityLaziest
-             (K : Component -> Prop)
-             (MCP:@MCPTrace context) : Prop :=
-    forall m c p m' MCP' MCP'' MO MO',
-      Last MCP (m,c,p) ->
-      rollback m (mstate (head MCP)) K m' ->
-      WithContextMP updateC c (MPTraceOf (m,p)) MCP' ->
-      WithContextMP updateC c (MPTraceOf (m',p)) MCP'' ->
-      ObsOfMCP MCP' MO ->
-      ObsOfMCP MCP'' MO' ->
-      ObsOfMP MO ~=_O ObsOfMP MO'.
+    Variable context : Type.
+    Variable updateC : MachineState -> context -> context.
 
-  (* The second property identifies the subset of protected components that
-     changed between the beginning and the end of the trace. The property holds
-     if that subset remains confidential permanently, defined in terms of trace
-     confidentiality holding on the trace from the final state.*)
-  Definition TraceIntegrityLazy
-             (K : Component -> Prop)
-             (MCP:@MCPTrace context) : Prop :=
-    forall m c p MCP',
-      Last MCP (m,c,p) ->
-      let K' := fun k => K k /\ mstate (head MCP) k <> mstate (m,c,p) k in
-      let P := fun _ _ => False in
-      WithContextMP updateC c (MPTraceOf (m,p)) MCP' ->
-      TraceConfidentialityEager updateC K' P MCP'.
+    Definition rollback (m m':MachineState) (K : Component -> Prop) (m'': MachineState) : Prop :=
+      forall k,
+        K k ->
+        proj m k <> proj m' k ->
+        proj m'' k = proj m k /\
+        (K k \/ proj m k = proj m' k) ->
+        proj m'' k = proj m' k.
 
-  (* Distinguishing example
-     f() {
-       int x = 0;
-       g();
-       if(x)
-         print x;
-       else
-         print 1;
-     }
+    Definition TraceIntegrityLaziest
+               (K : Component -> Prop)
+               (MPC:@MPCTrace context) : Prop :=
+      forall m p c m' Om On K,
+        Last MPC (m,p,c) ->
+        rollback (mstate (head MPC)) m K m' ->
+        ObsOfMPC updateC (MPCTraceOf updateC (m,p,c)) Om ->
+        ObsOfMPC updateC (MPCTraceOf updateC (m',p,c)) On ->
+        Om ~=_O On.
 
-     g() {
-       x = 1 // through arithmetic from the stack pointer, set x to 1
-     }
-   *)
+    (* The second property identifies the subset of protected components that
+       changed between the beginning and the end of the trace. The property holds
+       if that subset remains confidential permanently, defined in terms of trace
+       confidentiality holding on the trace from the final state.*)
+    Definition TraceIntegrityLazy
+               (K : Component -> Prop)
+               (MPC:@MPCTrace context) : Prop :=
+      forall m p c,
+        Last MPC (m,p,c) ->
+        let K' := fun k => K k /\ proj (mstate (head MPC)) k <> proj (mstate (m,p,c)) k in
+        let P := fun _ => False in
+        TraceConfidentialityEager updateC K' P (MPCTraceOf updateC (m,p,c)).
 
+    (* Distinguishing example
+       f() {
+         int x = 0;
+         g();
+         if(x)
+           print x;
+         else
+           print 1;
+       }
 
-End LAZY_TRACE_PROPS.
+       g() {
+         x = 1 // through arithmetic from the stack pointer, set x to 1
+       }
+     *)
 
-Section WITH_MAPS.
+    (* Policy-aware (testable) property *)
+    Variable DeadCrit : MPState -> Component -> Prop.
+    Definition ReallyDead (DeadCrit : MPState -> Component -> Prop) : Prop :=
+      forall mp c,
+        let K := fun k => DeadCrit mp k in
+        let P := fun _ => False in
+        TraceConfidentialityEager updateC K P (MPCTraceOf updateC (mp,c)).
 
-  Variable cdm : CodeMap'.
-  Variable sm : StackMap.
-  Variable pOf : MachineState -> PolicyState.
+    Definition IntegrityOrDeath
+               (DeadCrit : MPState -> Component -> Prop)
+               (K : Component -> Prop)
+               (MPC:@MPCTrace context) : Prop :=
+      forall m p c k,
+        Last MPC (m,p,c) ->
+        K k ->
+        proj (mstate (head MPC)) k = proj (mstate (m,p,c)) k \/ DeadCrit (m,p) k.
 
-  Definition SealingConvention : Type := MachineState -> Addr -> bool.
-  Variable sc : SealingConvention.
+    Theorem TraceIntegrityDeadLazy :
+      forall K MPC,
+        ReallyDead DeadCrit ->
+        IntegrityOrDeath DeadCrit K MPC ->
+        TraceIntegrityLazy K MPC.
+    Proof.
+      unfold TraceIntegrityLazy.
+      unfold ReallyDead.
+      unfold TraceConfidentialityEager.
+      intros. specialize H with (m,p) MPC0 m0 c0 p0 n N Om On.
+      apply (H c H2); auto.
+      unfold variantOf. intros.
+      apply H3. intro. destruct H8.
+      unfold IntegrityOrDeath in H0.
+      specialize H0 with m p c k. apply H0 in H1; auto. destruct H1; auto.
+    Qed.
 
-  Definition context : Type := DomainMap * DepthMap.
+    Definition UltraDead (DeadCrit : MPState -> Component -> Prop) : Prop :=
+      forall m n p m' n' p' p'' o o',
+        let K := fun k => DeadCrit (m,p) k in
+        variantOf K m n ->
+        mpstep (m,p) = Some (m',p',o) ->
+        mpstep (n,p) = Some (n',p'',o') ->
+        forall k,
+          proj m' k <> proj n' k ->
+          DeadCrit (m',p') k /\ DeadCrit (n',p') k.
+
+    Theorem UltraDeadIsReallyDead :
+      UltraDead DeadCrit -> ReallyDead DeadCrit.
+    Proof.
+      unfold UltraDead. unfold ReallyDead.
+      unfold TraceConfidentialityEager. intros.
+    Admitted.
+      
+      
+  End LAZY_TRACE_PROPS.
+
+  (* We add coroutines with multiple stacks, defined with static extents (see Machine.v).
+     Our domain model uses the same stack domain as previous, but now a top-level domain
+     combines a stack identity and the domains of that stack. Outside is now a top domain. *)
+  Section DOMAIN_MODEL.
+
+    Inductive StackDomain :=
+    | Sealed (d:nat)
+    | Shared (d:nat)
+    | Passed (d:nat)
+    | Unsealed
+    .
+
+    Inductive TopDomain :=
+    | Instack (sid:StackID) (sd:StackDomain)
+    | Outside
+    .
+
+    Definition DomainMap := Component -> TopDomain.
+
+    (* We will additionally track the depths of all the stack simultaneously. *)
+    Definition DepthMap := StackID -> nat.
+    Definition initDepM : DepthMap := fun sid => O.
+    Definition push (depm: DepthMap) (sid: StackID) :=
+      fun sid' => if stack_eqb sid sid'
+                  then (depm sid)+1
+                  else depm sid.
+    Definition pop (depm: DepthMap) (sid: StackID) :=
+      fun sid' => if stack_eqb sid sid'
+                  then (depm sid)-1
+                  else depm sid.
   
-  Definition initC : DomainMap * DepthMap :=
-    let dm := fun k =>
-                match k with
-                | Mem a =>
-                  match findStack sm a with
-                  | Some sid => Instack sid Unsealed
-                  | None => Outside
-                  end
-                | Reg r => Outside
-                end in
-    (dm,initDepM).
+  End DOMAIN_MODEL.
+
+  Section WITH_MAPS.
+
+    Variable cdm : CodeMap.
+    Variable sm : StackMap.
+
+    Definition SealingConvention : Type := MachineState -> Addr -> bool.
+    Variable sc : SealingConvention.
+
+    Definition context : Type := DomainMap * DepthMap.
   
-  (* Once again we need an update function for out context. Note that yields don't
-     actually change the domain map, as they don't change which addresses belong to which
-     stacks. So we still only consider sharing, calls, and returns. *)
-  Definition updateC (m:MachineState) (prev:context) : context :=
-    let '(dm, depm) := prev in
-    let sid := activeStack sm m in
-    let d := depm sid in
-    match AnnotationOf cdm (m (Reg PC)) with
-    | Some (share f) =>
-      let dm' := fun k =>
-                   match k with
-                   | Mem a =>
-                     match f m a, dm k with
-                     | Some true, Instack sid' Unsealed =>
-                       if stack_eqb sid sid' 
-                       then Instack sid (Passed d)
-                       else dm k
-                     | Some false, Instack sid' Unsealed =>
-                       if stack_eqb sid sid' 
-                       then Instack sid (Shared d)
-                       else dm k
-                     | _, _ => dm k
-                     end
-                   | _ => dm k
-                   end in
-      (dm', depm)
-    | Some call =>
-      let dm' := fun k =>
-                    match k, dm k with                      
-                    | _, Instack sid' (Sealed d) => Instack sid' (Sealed d)
-                    | _, Outside => Outside
-                    | Mem a, Instack sid' _ =>
-                      if sc m a && stack_eqb sid sid'
-                      then Instack sid (Sealed d)
-                      else Instack sid Unsealed (* If addresses are marked to be shared but the sealing convention
-                                       wants them unsealed, the sealing convention takes precedence *)
-                    | _, _ => dm k
-                    end in
-      (dm', push depm sid)
-    | Some ret => 
-      let dm' := fun k =>
-                    match dm k with
-                    | Instack sid' (Sealed d') =>
-                      if (d-1 =? d') && stack_eqb sid sid'
-                      then Instack sid Unsealed
-                      else dm k
-                    | Instack sid' (Passed d') =>
-                      if (d-1 =? d') && stack_eqb sid sid'
-                      then Instack sid Unsealed
-                      else dm k
-                    | Instack sid' (Shared d') =>
-                      if (d =? d') && stack_eqb sid sid'
-                      then Instack sid Unsealed
-                      else dm k
-                    | _ => dm k
-                    end in
-      (dm', pop depm sid)
-    | _ => (dm, depm)
-    end.
-
-  Definition StackInaccessible (c:context) (k:Component) : Prop :=
-    exists sid d,
-      fst c k = Instack sid (Sealed d) \/
-      (fst c k = Instack sid (Passed d) /\ d < (snd c sid)-1).
-
-  (* We split up our inaccessibility criterion into stack and coroutine variations.
-     The coroutine version takes the active stack, and prohibits accessing other stacks
-     except for shared objects. *)
-  Definition CoroutineInaccessible (c:context) (sid:StackID) (k:Component) : Prop :=
-    forall sid' sd d,
-      fst c k = Instack sid' sd ->
-      (sid <> sid /\ sd <> Shared d).
+    Definition initC : DomainMap * DepthMap :=
+      let dm := fun k =>
+                  match k with
+                  | Mem a =>
+                    match sm a with
+                    | Some sid => Instack sid Unsealed
+                    | None => Outside
+                    end
+                  | Reg r => Outside
+                  | PC => Outside
+                  end in
+      (dm,initDepM).
   
-  (* We presumably want a Yield Rule that is equivalent to the Call Rule. *)
-(*  Definition YieldRule : Prop :=
-    forall minit MCP sid my cy py mp o m' c' p' MCP',
-      WithContextMP updateC initC (MPTraceOf (minit, pOf minit)) MCP ->
-      InTrace (my,cy,py) MCP -> (* From any state that is a yield *)
-      AnnotationOf cdm (my (Reg PC)) = Some yield -> (* As determined by the code annotations *)
-      activeStack sm my = sid -> (* With active stack sid *)
-      mpstep (my,py) = Some (mp,o) -> (* That has a successful step, i.e. doesn't immediately fail-stop *)
+    (* Once again we need an update function for out context. Note that yields don't
+       actually change the domain map, as they don't change which addresses belong to which
+       stacks. So we still only consider sharing, calls, and returns. *)
+    Definition updateC (m:MachineState) (prev:context) :
+      context :=
+      let '(dm, depm) := prev in
+      match activeStack sm m with
+      | None => prev (* Shouldn't happen *)
+      | Some sid => 
+        let d := depm sid in
+        match AnnotationOf cdm (proj m PC) with
+        | Some (share f) =>
+          let dm' := fun k =>
+                       match k with
+                       | Mem a =>
+                         match f m a, dm k with
+                         | Some true, Instack sid' Unsealed =>
+                           if stack_eqb sid sid' 
+                           then Instack sid (Passed d)
+                           else dm k
+                         | Some false, Instack sid' Unsealed =>
+                           if stack_eqb sid sid' 
+                           then Instack sid (Shared d)
+                           else dm k
+                         | _, _ => dm k
+                         end
+                       | _ => dm k
+                       end in
+          (dm', depm)
+        | Some call =>
+          let dm' := fun k =>
+                       match k, dm k with                      
+                       | _, Instack sid' (Sealed d) => Instack sid' (Sealed d)
+                       | _, Outside => Outside
+                       | Mem a, Instack sid' _ =>
+                         if sc m a && stack_eqb sid sid'
+                         then Instack sid (Sealed d)
+                         else Instack sid Unsealed (* If addresses are marked to be shared but the sealing convention
+                                                      wants them unsealed, the sealing convention takes precedence *)
+                       | _, _ => dm k
+                       end in
+          (dm', push depm sid)
+        | Some ret => 
+          let dm' := fun k =>
+                       match dm k with
+                       | Instack sid' (Sealed d') =>
+                         if (d-1 =? d') && stack_eqb sid sid'
+                         then Instack sid Unsealed
+                         else dm k
+                       | Instack sid' (Passed d') =>
+                         if (d-1 =? d') && stack_eqb sid sid'
+                         then Instack sid Unsealed
+                         else dm k
+                       | Instack sid' (Shared d') =>
+                         if (d =? d') && stack_eqb sid sid'
+                         then Instack sid Unsealed
+                         else dm k
+                       | _ => dm k
+                       end in
+          (dm', pop depm sid)
+        | _ => (dm, depm)
+        end
+      end.
 
-      (* We can look ahead to the next state whose stack is sid *)
-      FindSegmentMP updateC (fun m c => activeStack sm m <> sid) mp (updateC my cy) MCP' ->
-      Last MCP' (m',c',p') ->
-      (* And that state will maintain the values of all addresses in sid. *)
-      forall a sd,
-        fst cy (Mem a) = Instack sid sd ->
-        my (Mem a) = m' (Mem a).      
-*)  
-  Definition StackIntegrityLazy : Prop :=
-    forall minit MCP sid d,
-      let P := fun m (c:context) => snd c sid = d in
-      FindSegmentMP updateC P (minit, pOf minit) initC MCP ->
-      TraceIntegrityLazy context updateC (StackInaccessible (cstate (head MCP))) MCP.
+    Definition StackInaccessible (c:context) (k:Component) : Prop :=
+      exists sid d,
+        fst c k = Instack sid (Sealed d) \/
+        (fst c k = Instack sid (Passed d) /\ d < (snd c sid)-1).
+    
+    (* We split up our inaccessibility criterion into stack and coroutine variations.
+       The coroutine version takes the active stack, and prohibits accessing other stacks
+       except for shared objects. *)
+    Definition CoroutineInaccessible (c:context) (sid:StackID) (k:Component) : Prop :=
+      forall sid' sd d,
+        fst c k = Instack sid' sd ->
+        (sid <> sid /\ sd <> Shared d).
 
-  Definition CoroutineIntegrityLazy : Prop :=
-    forall minit MCP sid,
-      FindSegmentMP updateC (fun m c => activeStack sm m = sid) (minit, pOf minit) initC MCP ->
-      TraceIntegrityLazy context updateC (fun k => CoroutineInaccessible (cstate (head MCP)) sid k) MCP.
-
-  (* We can do a confidentiality rule similarly *)
-  Definition YieldConfRule : Prop :=
-    forall minit MCP sid my cy py m p o n MCP' N MO NO,
-      WithContextMP updateC initC (MPTraceOf (minit, pOf minit)) MCP ->
-      InTrace (my,cy,py) MCP -> (* Once again we consider each successful call *)
-      AnnotationOf cdm (my (Reg PC)) = Some yield ->
-      mpstep (my,py) = Some (m,p,o) ->
-
-      (* And take any variant state of the first state within it *)
-      variantOf (fun k => forall sd, fst cy k <> Instack sid sd) m n ->
-      (* If we trace from both states until they each return... *)
-      FindSegmentMP updateC (fun m c => activeStack sm m <> sid) (m,p) cy MCP' ->
-      FindSegmentMP updateC (fun m c => activeStack sm m <> sid) (n,p) cy N ->
-      (* They should have the same observable behavior *)
-      ObsOfMCP MCP' MO ->
-      ObsOfMCP N NO ->
-      ObsOfMP MO ~=_O ObsOfMP NO /\
-      (* And when they return, the states should have changed in identical ways. *)
-      (forall m' c' p',
-          Last MCP' (m',c',p') ->
-          exists n' c'',
-            Last N (n',c'',p') /\
-            sameDifference my m' n n').
+    Definition StackIntegrityUE : Prop :=
+      forall k m c p m' p' c' o,
+        Reachable updateC initC (m,p,c) ->
+        mpcstep updateC (m,p,c) = Some (m',p',c',o) ->
+        StackInaccessible c k ->
+        proj m k = proj m' k.
   
-  Definition StackConfidentialityEager : Prop :=
-    forall minit MCP d sid,
-      let P := (fun m c => snd c sid = d) in
-      let K := (fun k => StackInaccessible (cstate (head MCP)) k \/
-                         fst (cstate (head MCP)) k = Instack sid Unsealed) in
-      FindSegmentMP updateC P (minit, pOf minit) initC MCP ->
-      TraceConfidentialityEager updateC K P MCP.
+    Definition CoroutineIntegrityUE : Prop :=
+      forall sid k m c p m' p' c' o,
+        Reachable updateC initC (m,p,c) ->
+        mpcstep updateC (m,p,c) = Some (m',p',c',o) ->
+        CoroutineInaccessible c sid k ->
+        proj m k = proj m' k.
+    
+    (* We can actually do ultra eager confidentiality for coroutines without any more complexity,
+       because coroutine properties don't care about allocation and initialization. That only comes
+       when subroutine properties are layered in. *)
+    Definition SealedConfidentialityUE : Prop :=
+      forall sid m p c m' p' c' n o n' p'' c'' o',
+        Reachable updateC initC (m,p,c) ->
+        mpcstep updateC (m,p,c) = Some (m',p',c',o) ->
+        variantOf (fun k => CoroutineInaccessible c sid k) m n ->
+        mpcstep updateC (n,p,c) = Some (n',p'',c'',o') ->
+        sameDifference m m' n n' /\ p' = p'' /\ o = o'.
 
-  Definition CoroutineConfidentialityEager : Prop :=
-    forall minit MCP sid,
-      let P := (fun m c => activeStack sm m = sid) in
-      let K := (fun k => CoroutineInaccessible (cstate (head MCP)) sid k) in
-      FindSegmentMP updateC P (minit, pOf minit) initC MCP ->
-      TraceConfidentialityEager updateC K P MCP.
+    Definition StackIntegrityEager : Prop :=
+      forall MCP sid d,
+        ReachableSegment updateC initC (fun '(m,p,c) => snd c sid >= d) MCP ->
+        TraceIntegrityEager (StackInaccessible (cstate (head MCP))) MCP.
 
-  (* ***** Control Flow Properties ***** *)
-
-
-  (* Finally, we also need to consider control flow properties. These are included here because
-     they don't really change in interesting ways between the different models. *)
+    Definition CoroutineIntegrityEager : Prop :=
+      forall MCP sid,
+        ReachableSegment updateC initC (fun '(m,p,c) => activeStack sm m = Some sid) MCP ->
+        TraceIntegrityEager (fun k => CoroutineInaccessible (cstate (head MCP)) sid k) MCP.
+    
+    Definition StackConfidentialityEager : Prop :=
+      forall sid MCP d m dm depm p,
+        let P := (fun '(m,p,c) => snd c sid >= d) in
+        let K := (fun k => StackInaccessible (cstate (head MCP)) k \/
+                           fst (cstate (head MCP)) k = Instack sid Unsealed) in
+        ReachableSegment updateC initC P MCP ->
+        head MCP = (m,p,(dm,depm)) ->
+        TraceConfidentialityEager updateC K P MCP.
   
-  Definition ControlSeparation : Prop :=
-    forall minit m1 p1 m2 p2 o f1 f2 ann1 ann2,
+    Definition CoroutineConfidentialityEager : Prop :=
+      forall MCP sid,
+        let P := (fun '(m,p,c) => activeStack sm m = Some sid) in
+        let K := (fun k => CoroutineInaccessible (cstate (head MCP)) sid k) in
+        ReachableSegment updateC initC P MCP ->
+        TraceConfidentialityEager updateC K P MCP.
+
+    (* ***** Control Flow Properties ***** *)
+
+
+    (* Finally, we also need to consider control flow properties. These are included here because
+       they don't really change in interesting ways between the different models. *)
+  
+    (*Definition ControlSeparation : Prop :=
+      forall minit m1 p1 m2 p2 o f1 f2 ann1 ann2,
       InTrace (m1,p1) (MPTraceOf (minit, pOf minit)) ->
       mpstep (m1,p1) = Some (m2, p2,o) ->
-      cdm (m1 (Reg PC)) = inFun f1 ann1 ->
-      cdm (m2 (Reg PC)) = inFun f2 ann2 ->
+      cdm (proj m1 PC) = inFun f1 ann1 ->
+      cdm (proj m2 PC) = inFun f2 ann2 ->
       f1 <> f2 ->
-      AnnotationOf cdm (m1 (Reg PC)) = Some call \/
-      AnnotationOf cdm (m1 (Reg PC)) = Some ret \/
-      AnnotationOf cdm (m1 (Reg PC)) = Some yield.
+      AnnotationOf cdm (proj m1  PC) = Some call \/
+      AnnotationOf cdm (proj m1  PC) = Some ret \/
+      AnnotationOf cdm (proj m1  PC) = Some yield. *)
 
-  Definition YieldBackIntegrity : Prop :=
-    forall mp mp1 mp2 MPout,
-      InTrace mp1 (MPTraceOf mp) ->
-      AnnotationOf cdm (ms mp1 (Reg PC)) = Some yield ->
-      SplitInclusive (fun mp2 => sm (ms mp1 (Reg SP)) = sm (ms mp (Reg SP))) (MPTraceOf mp) MPout (MPTraceOf mp2) ->
-      justRet (ms mp1) (ms mp2).
+    Definition YieldBackIntegrity : Prop :=
+      forall mpc1 mpc2,
+        let P := (fun mpc => sm (proj (mstate mpc1) (Reg SP)) = sm (proj (mstate mpc) (Reg SP))) in
+        Reachable updateC initC mpc1 ->
+        AnnotationOf cdm (proj (mstate mpc1) PC) = Some yield ->
+        StepsToWhen updateC P mpc1 mpc2 ->
+        justRet (mstate mpc1) (mstate mpc2).
 
-  Definition ReturnIntegrity : Prop :=
-    forall sid d minit MCP m c p m' c' p',
-      let P := fun m c => activeStack sm m = sid /\ (snd c) sid >= d in
-      FindSegmentMP updateC P (minit, pOf minit) initC MCP ->
-      head MCP = (m,c,p) ->
-      Last MCP (m',c',p') ->
-      justRet m m'.
-
-  Variable em:EntryMap.
+    Definition ReturnIntegrity : Prop :=
+      forall d sid MCP m c p m' c' p',
+        let P := fun '(m,p,c) => activeStack sm m = Some sid /\ (snd c) sid >= d in
+        ReachableSegment updateC initC P MCP ->
+        head MCP = (m,c,p) ->
+        Last MCP (m',c',p') ->
+        justRet m m'.
   
-  Definition EntryIntegrity : Prop :=
-  forall minit mp1 m2 p2 o,
-    InTrace mp1 (MPTraceOf (minit, pOf minit)) ->
-    mpstep mp1 = Some (m2,p2,o) ->
-    AnnotationOf cdm (ms mp1 (Reg PC)) = Some call ->
-    em (m2 (Reg PC)).
+    Variable em:EntryMap.
 
-  Definition WellBracketedControlFlow  : Prop :=
-    ControlSeparation /\
-    ReturnIntegrity /\
-    YieldBackIntegrity /\
-    EntryIntegrity.
+    Definition EntryIntegrity : Prop :=
+      forall mpc1 mpc2 o,
+        Reachable updateC initC mpc1 ->
+        mpcstep updateC mpc1 = Some (mpc2,o) ->
+        AnnotationOf cdm (proj (mstate mpc1) PC) = Some call ->
+        em (proj (mstate mpc2) PC) = true.
 
-  (* Next check out lazy.v for lazy properties *)
+    Definition WellStructuredControlFlow  : Prop :=
+      (*ControlSeparation /\ *)
+      ReturnIntegrity /\
+      YieldBackIntegrity /\
+      EntryIntegrity.
 
-End WITH_MAPS.
+  End WITH_MAPS.
