src/TraceProperties.v
@@ -4,17 +4,17 @@ Require Import Bool.
 
 From StackSafety Require Import Trace Machine ObsTrace.
 
-
-  Section WITH_CONTEXT.
+Section WITH_CONTEXT.
 
   Variable context : Type.
   Variable updateC : MachineState -> context -> context.
 
-  Definition TraceIntegrityEager (K : Component -> Prop) (MPC:MPCTrace) : Prop :=
+  (* Not really using this one.*)
+(*  Definition TraceIntegrityEager (K : Component -> Prop) (MPC:MPCTrace) : Prop :=
     forall k (mcp':@MPCState context),
       K k->
       Last MPC mcp' ->
-      proj (mstate (head MPC)) k = proj (mstate mcp') k.
+      proj (mstate (head MPC)) k = proj (mstate mcp') k.*)
   
   Definition variantOf (K : Component -> Prop) (m n : MachineState) :=
     forall k, ~ K k -> proj m k = proj n k.
@@ -23,8 +23,67 @@ From StackSafety Require Import Trace Machine ObsTrace.
     forall k,
       (proj m k <> proj m' k \/ proj n k <> proj n' k) ->
       proj m' k = proj n' k.
-  
-  Definition TraceConfidentialityEager
+
+  Inductive Lockstep : @MPCTrace context -> @MPCTrace context -> Prop :=
+  | bothDone : forall m p c n,
+      Lockstep (finished (m,p,c)) (finished (n,p,c))
+  | bothStep : forall m p c m' n n' M N,
+      mstate (head M) = m' ->
+      mstate (head N) = n' ->
+      sameDifference m m' n n' ->
+      Lockstep M N ->
+      Lockstep (notfinished (m,p,c) M) (notfinished (n,p,c) N)
+  .
+
+  Definition TraceConfidentialityStep
+             (K : Component -> Prop)
+             (P : MPCState -> Prop)
+             (M : @MPCTrace context) : Prop :=
+    forall m p c n N,
+      head M = (m,p,c) ->
+      variantOf K m n ->
+      MPCTraceToWhen updateC P (n,p,c) N ->
+      Lockstep M N
+  .
+
+  Definition StepIntegrity (K : Component -> Prop) (mpc:@MPCState context) : Prop :=
+    forall mpc' o k,
+    mpcstep updateC mpc = Some (mpc',o) ->
+    K k ->
+    proj (mstate mpc) k = proj (mstate mpc') k.
+
+  Definition TraceIntegrityLazy
+             (K : Component -> Prop)
+             (M : @MPCTrace context) : Prop :=
+    forall m p c,
+      Last M (m,p,c) ->
+      let K' := fun k => K k /\ proj (mstate (head M)) k <> proj (mstate (m,p,c)) k in
+      let P := fun _ => False in
+      TraceConfidentialityStep K' P (MPCTraceOf updateC (m,p,c)).
+
+  Definition TraceConfidentialityLazy
+             (K : Component -> Prop)
+             (P : MPCState -> Prop)
+             (M : @MPCTrace context) : Prop :=
+    forall m p c n N,
+      head M = (m,p,c) ->
+      variantOf K m n ->
+      MPCTraceToWhen updateC P (n,p,c) N ->
+      (exists mend nend pend cend,
+          Last M (mend,pend,cend) /\
+          Last N (nend,pend,cend) /\
+          P (mend,pend,cend) /\
+          P (nend,pend,cend) /\
+          let K := fun k => mend <> nend in
+          TraceConfidentialityStep K P (MPCTraceOf updateC (mend,pend,cend))) \/
+      (exists mpcend npcend,
+          Last M mpcend /\
+          Last N npcend /\
+          ~ P mpcend /\
+          ~ P npcend) \/
+      (Infinite M /\ Infinite N).
+
+(*Definition TraceConfidentialityEager
              (K : Component -> Prop)
              (P: MPCState -> Prop)
              (MPC:@MPCTrace context) : Prop :=
@@ -34,25 +93,26 @@ From StackSafety Require Import Trace Machine ObsTrace.
       MPCTraceToWhen updateC P (n,c,p) N ->
       ObsOfMPC updateC MPC Om ->
       ObsOfMPC updateC N On ->
-      (* Case 1 *)
-      (forall mpcend,
-          Last MPC mpcend ->
-          ~ P mpcend ->
-          exists npcend,
-            Last N npcend /\
-            Om ~=_O On /\
-            sameDifference m (mstate mpcend) n (mstate npcend))
-    /\ (* Case 2 *)
-    (Infinite MPC ->
-     Om ~=_O On)
-    /\ (* Case 3 *)
-    (forall mpcend,
-        Last MPC mpcend ->
-        P mpcend ->
-        Om <=_O On).
 
+      Om ~=_O On /\
+
+      ((exists mpcend npcend,
+          Last MPC mpcend /\
+          Last N npcend /\
+          P mpcend /\
+          P npcend /\
+          sameDifference m (mstate mpcend) n (mstate npcend)) \/
+      (Infinite MPC /\ Infinite N) \/
+      (exists mpcend npcend,
+          Last MPC mpcend /\
+          Last N npcend /\
+          ~ P mpcend /\
+          ~ P npcend)). *)
+      
 End WITH_CONTEXT.
 
-Arguments TraceIntegrityEager {_} _ _.
-Arguments TraceConfidentialityEager {_} _ _ _ _.
+Arguments StepIntegrity {_} _ _.
+Arguments TraceConfidentialityStep {_} _ _ _ _.
+Arguments TraceIntegrityLazy {_} _ _.
+Arguments TraceConfidentialityLazy {_} _ _ _ _.
 
